operational_semantics/operational_semantics.v
@@ -5,53 +5,53 @@ Add LoadPath "C:\Users\Ziga\Documents\Ziga_podatki\repositories\eeff-formalizati
 Require Export syntax substitution.
 
 Inductive step : comp -> comp -> Prop :=
-| Step_ΠMatch v1 v2 x y c: 
+| Step_ΠMatch v1 v2 c: 
     step 
-      (ΠMatch (Pair v1 v2) x y c)
+      (ΠMatch (Pair v1 v2) c)
       (c_subs2_out c v1 v2)
-| Step_ΣMatch_Inl v x c1 y c2:
+| Step_ΣMatch_Inl v c1 c2:
     step 
-      (ΣMatch (Inl v) x c1 y c2)
+      (ΣMatch (Inl v) c1 c2)
       (c_subs_out c1 v)
-| Step_ΣMatch_Inr v x c1 y c2:
+| Step_ΣMatch_Inr v c1 c2:
     step 
-      (ΣMatch (Inr v) x c1 y c2)
+      (ΣMatch (Inr v) c1 c2)
       (c_subs_out c2 v)
-| Step_ListMatch_Nil c1 x xs c2:
+| Step_ListMatch_Nil c1 c2:
     step 
-      (ListMatch ListNil c1 x xs c2)
+      (ListMatch ListNil c1 c2)
       c1
-| Step_ListMatch_Cons v vs c1 x xs c2:
+| Step_ListMatch_Cons v vs c1 c2:
     step 
-      (ListMatch (ListCons v vs) c1 x xs c2)
+      (ListMatch (ListCons v vs) c1 c2)
       (c_subs2_out c2 v vs)
-| Step_App x c v:
-    step (App (Fun x c) v) (c_subs_out c v)
-| Step_LetRec f x c1 c2:
+| Step_App c v:
+    step (App (Fun c) v) (c_subs_out c v)
+| Step_LetRec c1 c2:
     step
-      (LetRec f x c1 c2)
-      (c_subs_out c2 (Fun x (LetRec f x (Sub.c_shift c1 1 2) c1)))
-| Step_DoBind_step x c1 c1' c2:
+      (LetRec c1 c2)
+      (c_subs_out c2 (Fun (LetRec (c_shift c1 1 2) c1)))
+| Step_DoBind_step c1 c1' c2:
     step c1 c1' ->
-    step (DoBind x c1 c2) (DoBind x c1' c2)
-| Step_DoBind_Ret x v c:
-    step (DoBind x (Ret v) c) (c_subs_out c v)
-| Step_DoBind_Op x op_id v_arg y c1 c2:
+    step (DoBind c1 c2) (DoBind c1' c2)
+| Step_DoBind_Ret v c:
+    step (DoBind (Ret v) c) (c_subs_out c v)
+| Step_DoBind_Op op v c1 c2:
     step
-      (DoBind x (Op op_id v_arg y c1) c2)
-      (Op op_id v_arg y (DoBind x c1 (Sub.c_shift c2 1 1)))
+      (DoBind (Op op v c1) c2)
+      (Op op v (DoBind c1 (c_shift c2 1 1)))
 | Step_Handle_Step v c c' :
     step c c' ->
     step (Handle v c) (Handle v c')
-| Step_Handle_Ret x c_r h v :
+| Step_Handle_Ret c_r h v :
     step
-      (Handle (Handler x c_r h) (Ret v))
+      (Handle (Handler c_r h) (Ret v))
       (c_subs_out c_r v)
-| Step_Handle_Op x c_r h op_id v_arg y c_k x_op k_op c_op :
-    find_case h op_id = Some (x_op, k_op, c_op) ->
+| Step_Handle_Op c_r h op v c_k c_op :
+    find_case h op = Some c_op ->
     step
-      (Handle (Handler x c_r h) (Op op_id v_arg y c_k))
+      (Handle (Handler c_r h) (Op op v c_k))
       (c_subs2_out c_op
-        (Fun y (Handle (Sub.v_shift (Handler x c_r h) 1 0) c_k))
-        v_arg )
+        (Fun (Handle (v_shift (Handler c_r h) 1 0) c_k))
+        v )
 .
